prove toDate equivalent to smod formulation; use optimized encoding in SymCC
Signed-off-by: Victor Nicolet <victornl@amazon.com>

cedar-lean/Cedar/Spec/Ext/Datetime.lean
@@ -269,9 +269,12 @@ public def durationSince (datetime other: Datetime) : Option Duration :=
   Int64.sub? datetime.val other.val
 
 public def toDate (datetime: Datetime) : Option Datetime :=
-  -- we want datetime - (datetime % MS_PER_DAY), where `%` has the semantics of `Int64.smod`
   let millisPerDayI64 := Int64.ofIntChecked MILLISECONDS_PER_DAY (by decide)
-  datetime? (datetime.val - Int64.smod datetime.val millisPerDayI64)
+  if datetime.val >= 0
+  then datetime? (millisPerDayI64 * (datetime.val.div millisPerDayI64))
+  else if datetime.val.mod millisPerDayI64 == 0
+       then datetime
+       else datetime? (((datetime.val.div millisPerDayI64) - 1) * millisPerDayI64)
 
 public def toTime (datetime: Datetime) : Duration :=
   let millisPerDayI64 := Int64.ofIntChecked MILLISECONDS_PER_DAY (by decide)
